reactiveness

theories/SinkTm.v
@@ -7,4 +7,25 @@ From Hammer Require Import
   Tactics.
 
 (* TODO: fix with definintion. *)
-Fixpoint sinkTm (p : prefix) : term := TmSink.
+Fixpoint sinkTm (p : prefix) : term :=
+    match p with
+        PfxOneEmp => TmSink
+      | PfxOneFull => TmSink
+      | PfxEpsEmp => TmSink
+      | PfxParPair p1 p2 => TmComma (sinkTm p1) (sinkTm p2)
+      | PfxCatFst p1 => sinkTm p1
+      | PfxCatBoth p1 p2 => sinkTm p2
+      | PfxSumEmp => TmSink
+      | PfxSumInl p => sinkTm p
+      | PfxSumInr p => sinkTm p
+      | PfxStarEmp => TmSink
+      | PfxStarDone => TmSink
+      | PfxStarFirst p1 => sinkTm p1
+      | PfxStarRest p1 p2 => sinkTm p2
+    end
+.
+
+Theorem sink_reactive : forall p, reactive (sinkTm p).
+Proof.
+induction p; sauto lq: on.
+Qed.
